untimed/CaseStudy/AutomatonExample.thy
@@ -21,15 +21,18 @@ fun myTransition :: "(State \<times>(channel \<rightharpoonup> nat event)) \<Rig
 "myTransition _ = (myState, tsynbOneTick c1)"
 
 lift_definition myAutomaton :: "(State, nat event) automaton" is "(myTransition, myState, tsynbOneTick c1, {c2}, {c1})"
-  apply(simp add: automaton_well_def)
-    sorry
+  by simp
 
 
 definition mySPF :: "nat event SPF" where
 "mySPF = H myAutomaton"
 
+lift_definition testInSb::"nat event SB" is "([c2 \<mapsto> <[Msg 3]>])"
+  apply(rule ubwellI, auto)
+    sorry
 
 (* TODO: final lemma over mySPF *) 
 
-
+lemma "ubGetCh c1\<cdot> (mySPF \<rightleftharpoons> testInSb) = <[\<surd>]>"
+  sorry
 end
